---
title: "Follow-Up Discussion Board"
author: "Leticia Salazar"
date: "5/6/2022"
output: html_document
---

```{r setup, include=FALSE}
knitr::opts_chunk$set(echo = TRUE)
```
$~$

### Follow-Up Discussion Board 

![](/Users/letiix3/Desktop/Data-605/Week-14/William_Aiken_Q26.png)

$~$

### My contribution:

#### A Taylor series centered at zero or a = 0

#### The alternation that William explained looks like this:

$f(0) = 1$

$f'(x) = -e^{-x}$

$f'(x) = -1$

$f''(x) = e^{-x}$

$f''(x) = 1$

$f'''(x) = -e^{-x}$

$f'''(x) = -1$

$f''''(x) = e^{-x}$

$f''''(x) = 1$

#### Therefore:

#### $\sum_{n=0}^\infty (-1)^n \frac{x^n}{n!}$

